README.md
@@ -4,6 +4,5 @@ several experiments on F * for the generation of (almost) automatic proofs
 ## todo : 
 1. AVL tree (done)
 2. Set and Map module (done)
-3. Binary Decision Diagram (typed in this case for more efficient memoization)
+3. Binary Decision Diagram (typed in this case for more efficient memoization) : apply + restrict + simplify
 4. eventualy a SAT solver
-5. a little SMT solver (linear algebra and non-interpreted functions and variables) but... it's realy hard
